Garden/OpenVM/Sha256/utils.v
@@ -1,4 +1,6 @@
 Require Import Garden.Plonky3.M.
+Require Import Garden.Plonky3.MExpr.
+Require Import OpenVM.primitives.utils.
 
 (* pub const SHA256_ROW_VAR_CNT: usize = 5; *)
 Definition SHA256_ROW_VAR_CNT : Z := 5.
@@ -17,3 +19,151 @@ Definition SHA256_WORD_U8S : Z := SHA256_WORD_BITS / 8.
 
 (* pub const SHA256_HASH_WORDS: usize = 8; *)
 Definition SHA256_HASH_WORDS : Z := 8.
+
+(*
+pub(crate) fn xor_bit<F: FieldAlgebra + Clone>(
+    x: impl Into<F>,
+    y: impl Into<F>,
+    z: impl Into<F>,
+) -> F {
+    let (x, y, z) = (x.into(), y.into(), z.into());
+    (x.clone() * y.clone() * z.clone())
+        + (x.clone() * not::<F>(y.clone()) * not::<F>(z.clone()))
+        + (not::<F>(x.clone()) * y.clone() * not::<F>(z.clone()))
+        + (not::<F>(x) * not::<F>(y) * z)
+}
+*)
+Definition xor_bit (x y z : Expr.t) : Expr.t :=
+  (x *E y *E z) +E
+  (x *E Expr.not y *E Expr.not z) +E
+  (Expr.not x *E y *E Expr.not z) +E
+  (Expr.not x *E Expr.not y *E z).
+
+(*
+pub(crate) fn xor<F: FieldAlgebra + Clone>(
+    x: &[impl Into<F> + Clone; SHA256_WORD_BITS],
+    y: &[impl Into<F> + Clone; SHA256_WORD_BITS],
+    z: &[impl Into<F> + Clone; SHA256_WORD_BITS],
+) -> [F; SHA256_WORD_BITS] {
+    array::from_fn(|i| xor_bit(x[i].clone(), y[i].clone(), z[i].clone()))
+}
+*)
+Definition xor (x y z : Array.t Expr.t SHA256_WORD_BITS) : Array.t Expr.t SHA256_WORD_BITS :=
+  {|
+    Array.get (i : Z) := xor_bit x.[i] y.[i] z.[i];
+  |}.
+
+(*
+pub(crate) fn rotr<F: FieldAlgebra + Clone>(
+    bits: &[impl Into<F> + Clone; SHA256_WORD_BITS],
+    n: usize,
+) -> [F; SHA256_WORD_BITS] {
+    array::from_fn(|i| bits[(i + n) % SHA256_WORD_BITS].clone().into())
+}
+*)
+Definition rotr (bits : Array.t Expr.t SHA256_WORD_BITS) (n : Z) :
+    Array.t Expr.t SHA256_WORD_BITS :=
+  {|
+    Array.get (i : Z) := bits.[(i + n) mod SHA256_WORD_BITS];
+  |}.
+
+(*
+pub(crate) fn shr<F: FieldAlgebra + Clone>(
+    bits: &[impl Into<F> + Clone; SHA256_WORD_BITS],
+    n: usize,
+) -> [F; SHA256_WORD_BITS] {
+    array::from_fn(|i| {
+        if i + n < SHA256_WORD_BITS {
+            bits[i + n].clone().into()
+        } else {
+            F::ZERO
+        }
+    })
+}
+*)
+Definition shr (bits : Array.t Expr.t SHA256_WORD_BITS) (n : Z) : Array.t Expr.t SHA256_WORD_BITS :=
+  {|
+    Array.get (i : Z) :=
+      if i + n <? SHA256_WORD_BITS then
+        bits.[i + n]
+      else
+        Expr.ZERO;
+  |}.
+
+(*
+pub(crate) fn small_sig0_field<F: FieldAlgebra + Clone>(
+    x: &[impl Into<F> + Clone; SHA256_WORD_BITS],
+) -> [F; SHA256_WORD_BITS] {
+    xor(&rotr::<F>(x, 7), &rotr::<F>(x, 18), &shr::<F>(x, 3))
+}
+*)
+Definition small_sig0_field (x : Array.t Expr.t SHA256_WORD_BITS) :
+    Array.t Expr.t SHA256_WORD_BITS :=
+  xor (rotr x 7) (rotr x 18) (shr x 3).
+
+(*
+pub(crate) fn small_sig1_field<F: FieldAlgebra + Clone>(
+    x: &[impl Into<F> + Clone; SHA256_WORD_BITS],
+) -> [F; SHA256_WORD_BITS] {
+    xor(&rotr::<F>(x, 17), &rotr::<F>(x, 19), &shr::<F>(x, 10))
+}
+*)
+Definition small_sig1_field (x : Array.t Expr.t SHA256_WORD_BITS) :
+    Array.t Expr.t SHA256_WORD_BITS :=
+  xor (rotr x 17) (rotr x 19) (shr x 10).
+
+(*
+pub fn constraint_word_addition<AB: AirBuilder>(
+    builder: &mut AB,
+    terms_bits: &[&[impl Into<AB::Expr> + Clone; SHA256_WORD_BITS]],
+    terms_limb: &[&[impl Into<AB::Expr> + Clone; SHA256_WORD_U16S]],
+    expected_sum: &[impl Into<AB::Expr> + Clone; SHA256_WORD_BITS],
+    carries: &[impl Into<AB::Expr> + Clone; SHA256_WORD_U16S],
+) {
+    for i in 0..SHA256_WORD_U16S {
+        let mut limb_sum = if i == 0 {
+            AB::Expr::ZERO
+        } else {
+            carries[i - 1].clone().into()
+        };
+        for term in terms_bits {
+            limb_sum += compose::<AB::Expr>(&term[i * 16..(i + 1) * 16], 1);
+        }
+        for term in terms_limb {
+            limb_sum += term[i].clone().into();
+        }
+        let expected_sum_limb = compose::<AB::Expr>(&expected_sum[i * 16..(i + 1) * 16], 1)
+            + carries[i].clone().into() * AB::Expr::from_canonical_u32(1 << 16);
+        builder.assert_eq(limb_sum, expected_sum_limb);
+    }
+}
+*)
+Definition constrain_word_addition
+    (terms_bits : list (Array.t Expr.t SHA256_WORD_BITS))
+    (terms_limb : list (Array.t Expr.t SHA256_WORD_U16S))
+    (expected_sum : Array.t Expr.t SHA256_WORD_BITS)
+    (carries : Array.t Expr.t SHA256_WORD_U16S) :
+    MExpr.t unit :=
+  MExpr.for_in_zero_to_n SHA256_WORD_U16S (fun i =>
+    let limb_sum : Expr.t :=
+      if i =? 0 then
+        Expr.ZERO
+      else
+        carries.[i - 1] in
+    let limb_sum : Expr.t :=
+      Lists.List.fold_left (fun limb_sum term =>
+        limb_sum +E utils.compose (Array.slice_range term (i * 16) ((i + 1) * 16)) 1
+      )
+      terms_bits
+      limb_sum in
+    let limb_sum : Expr.t :=
+      Lists.List.fold_left (fun limb_sum term =>
+        limb_sum +E term.[i]
+      )
+      terms_limb
+      limb_sum in
+    let expected_sum_limb : Expr.t :=
+      compose (Array.slice_range expected_sum (i * 16) ((i + 1) * 16)) 1 +E
+      carries.[i] *E Expr.from_canonical_u32 (2 ^ 16) in
+    MExpr.assert_eq limb_sum expected_sum_limb
+  ).
