Garden/OpenVM/primitives/utils.v
@@ -1,0 +1,17 @@
+Require Import Garden.Plonky3.M.
+Require Import Garden.Plonky3.MExpr.
+
+(*
+pub fn compose<F: FieldAlgebra>(a: &[impl Into<F> + Clone], limb_size: usize) -> F {
+    a.iter().enumerate().fold(F::ZERO, |acc, (i, x)| {
+        acc + x.clone().into() * F::from_canonical_usize(1 << (i * limb_size))
+    })
+}
+*)
+Definition compose {N : Z} (x : Array.t Expr.t N) (limb_size : Z) : Expr.t :=
+  Lists.List.fold_left (fun acc (i : nat) =>
+    let i : Z := Z.of_nat i in
+    acc +E x.[i] *E Expr.from_canonical_usize (2 ^ (i * limb_size))
+  )
+  (Lists.List.seq 0 (Z.to_nat N))
+  Expr.ZERO.
